@base  <http://www.idpf.org/epub/vocab/structure/> .
@prefix rdf:  <http://www.w3.org/1999/02/22-rdf-syntax-ns#> .
@prefix rdfs: <http://www.w3.org/2000/01/rdf-schema#> .
@prefix owl:  <http://www.w3.org/2002/07/owl#> .
@prefix zt:  <http://www.daisy.org/ns/rdf/property#> .
@prefix htu: <http://www.daisy.org/ns/rdf/usage/html/#> .
@prefix mou: <http://www.daisy.org/ns/rdf/usage/media-overlays/#> .
@prefix dcterms:  <http://purl.org/dc/terms/> .
@prefix jena: <http://www.daisy.org/ns/rdf/jena#> .
@prefix foaf: <http://xmlns.com/foaf/spec/#term_> .
@prefix aria: <http://www.w3.org/WAI/ARIA/schemata/aria-1.rdf#> .
@prefix xhv: <http://www.w3.org/1999/xhtml/vocab/#> .
@prefix role: <http://www.w3.org/1999/xhtml/vocab#> .
@prefix : <#> .

<>
  dcterms:title "EPUB 3 Structural Semantics Vocabulary" ;
  dcterms:description "This vocabulary, a part of EPUBÂ® 3, defines a set of properties relating to the description of structural semantics of written works. While the vocabulary is generally host language agnostic, it has been constructed primarily to enable semantic inflection of elements in the HTML vocabulary." ;
  dcterms:publisher "International Digital Publishing Forum (IDPF)" ;
  dcterms:issued "2011-05-06" ;  
  dcterms:creator "mgylling" ; 
  dcterms:creator "mgarrish" .
  

########## partitions #########

:partitions                             a rdf:Bag ;
					                       jena:bag-sort "10" ;
					                       dcterms:title "Document partitions" .
					
:cover                                  a rdf:Property ;
					                       rdfs:label "cover";
					                       rdf:member :partitions ;
					                       htu:usage "[[http://www.w3.org/TR/html5/sections.html#the-section-element section]]" ;
					                       jena:prop-sort "10" ;
					                       rdfs:comment "The publications cover(s), jacket information, etc." .							

:frontmatter                            a rdf:Property ;
					                       rdfs:label "frontmatter";
					                       rdf:member :partitions ;
					                       htu:usage "[[http://www.w3.org/TR/html5/sections.html#the-section-element section]]" ;
					                       jena:prop-sort "20" ;
					                       rdfs:comment "Preliminary material to the content body, such as tables of contents, dedications, etc." .

:bodymatter                             a rdf:Property ;
					                       rdfs:label "bodymatter";
					                       rdf:member :partitions ;
					                       htu:usage "[[http://www.w3.org/TR/html5/sections.html#the-section-element section]]" ;
					                       jena:prop-sort "30" ;
					                       rdfs:comment "The main (body) content of a document." .

:backmatter                             a rdf:Property ;
					                       rdfs:label "backmatter";
					                       rdf:member :partitions ;
					                       htu:usage "[[http://www.w3.org/TR/html5/sections.html#the-section-element section]]" ;
					                       jena:prop-sort "40" ;
					                       rdfs:comment "Ancillary material occurring after the document body, such as indices, appendices, etc." .



########## divisions #########

:divisions                              a rdf:Bag ;
                                            jena:bag-sort "20" ;
                                            dcterms:title "Document divisions" .

:volume                                 a rdf:Property ;
                                            rdfs:label "volume";
                                            rdf:member :divisions ;
                                            htu:usage "[[http://www.w3.org/TR/html5/sections.html#the-section-element section]]" ;
                                            jena:prop-sort "10" ;
                                            rdfs:comment "A component of a collection." .

:part                                   a rdf:Property;
                                            rdfs:label "part";
                                            rdf:member :divisions ;
                                            htu:usage "[[http://www.w3.org/TR/html5/sections.html#the-section-element section]]" ;
                                            jena:prop-sort "20" ;
                                            rdfs:comment "A major structural division of a piece of writing, typically encapsulating a set of related chapters." .

:chapter                                a rdf:Property ;
					                        rdfs:label "chapter";
                                            rdf:member :divisions ;
                                            htu:usage "[[http://www.w3.org/TR/html5/sections.html#the-section-element section]]" ;
                                            jena:prop-sort "30" ;
                                            rdfs:comment "A major structural division of a piece of writing." .

:subchapter                             a rdf:Property ;
                                            rdfs:label "subchapter";
                                            rdf:member :divisions ;
                                            htu:usage "[[http://www.w3.org/TR/html5/sections.html#the-section-element section]]" ;
                                            jena:prop-sort "40" ;
                                            rdfs:comment "A major sub-division of a chapter." .

:division                               a rdf:Property ;
                                            rdfs:label "division";
                                            rdf:member :divisions ;
                                            htu:usage "[[http://www.w3.org/TR/html5/sections.html#the-section-element section]]" ;
                                            jena:prop-sort "50" ;
                                            rdfs:comment "A major structural division that may also appear as a substructure of a part (esp. in legislation)." .

#:section                                a rdf:Property ;
#                                            rdfs:label "section";
#                                            rdf:member :divisions ;
#                                            rdfs:comment "A structural division typically subordinate in importance to a part or division (esp. in textbooks and legislation)." .
#
#:subsection                             a rdf:Property ;
#                                            rdfs:label "subsection";
#                                            rdf:member :divisions ;
#                                            rdfs:comment "A major sub-division of a section." .


########## sections #########

:sections                               a rdf:Bag ;
					                       jena:bag-sort "30" ;
					                       dcterms:title "Document sections and components" ;
					                       dcterms:description "Sections and components that typically occur in the publication bodymatter." .

:foreword                               a rdf:Property ;
                                            rdfs:label "foreword";
                                            rdf:member :sections ;
                                            htu:usage "[[http://www.w3.org/TR/html5/sections.html#the-section-element section]], [[http://www.w3.org/TR/html5/grouping-content.html#grouping-content grouping content]]" ;
                                            rdfs:comment "An introductory section that precedes the work, typically not written by the work's author." .

:preface                                a rdf:Property ;
                                            rdfs:label "preface";
                                            rdf:member :sections ;
                                            htu:usage "[[http://www.w3.org/TR/html5/sections.html#the-section-element section]], [[http://www.w3.org/TR/html5/grouping-content.html#grouping-content grouping content]]" ;
                                            rdfs:comment "An introductory section that precedes the work, typically written by the work's author." .

:prologue                               a rdf:Property ;
                                            rdfs:label "prologue" ;
                                            rdf:member :sections ;
                                            htu:usage "[[http://www.w3.org/TR/html5/sections.html#the-section-element section]], [[http://www.w3.org/TR/html5/grouping-content.html#grouping-content grouping content]]" ;
                                            rdfs:comment "An introductory section that sets the background to a story, typically part of the narrative." .

:introduction                           a rdf:Property ;
                                            rdfs:label "introduction";
                                            rdf:member :sections ;
                                            htu:usage "[[http://www.w3.org/TR/html5/sections.html#the-section-element section]], [[http://www.w3.org/TR/html5/grouping-content.html#grouping-content grouping content]]" ;
                                            rdfs:comment "A section in the beginning of the work, typically introducing the reader to the scope or nature of the work's content.".

:preamble                               a rdf:Property ;
                                            rdfs:label "preamble" ;
                                            rdf:member :sections ;
                                            htu:usage "[[http://www.w3.org/TR/html5/sections.html#the-section-element section]], [[http://www.w3.org/TR/html5/grouping-content.html#grouping-content grouping content]]" ;
                                            rdfs:comment "A section in the beginning of the work, typically containing introductory and/or explanatory prose regarding the scope or nature of the work's content".

:conclusion                             a rdf:Property ;
                                            rdfs:label "conclusion" ;
                                            rdf:member :sections ;
                                            htu:usage "[[http://www.w3.org/TR/html5/sections.html#the-section-element section]], [[http://www.w3.org/TR/html5/grouping-content.html#grouping-content grouping content]]" ;
                                            rdfs:comment "An ending section that typically wraps up the work." .

:epilogue                               a rdf:Property ;
                                            rdfs:label "epilogue" ;
                                            rdf:member :sections ;
                                            htu:usage "[[http://www.w3.org/TR/html5/sections.html#the-section-element section]], [[http://www.w3.org/TR/html5/grouping-content.html#grouping-content grouping content]]" ;
                                            rdfs:comment "A concluding section that is typically written from a later point in time than the main story, although still part of the narrative." .

:afterword		                        a rdf:Property ;
                                            rdfs:label "afterword" ;
                                            rdf:member :sections ;
                                            htu:usage "[[http://www.w3.org/TR/html5/sections.html#the-section-element section]], [[http://www.w3.org/TR/html5/grouping-content.html#grouping-content grouping content]]" ;
                                            rdfs:comment "An ending section that typically details the history of the story or its significance." .

:epigraph                               a rdf:Property ;
                                            rdfs:label "epigraph" ;
                                            rdf:member :sections ;
                                            htu:usage "[[http://www.w3.org/TR/html5/sections.html#the-section-element section]], [[http://www.w3.org/TR/html5/grouping-content.html#grouping-content grouping content]]" ;
                                            rdfs:comment "A quotation that is pertinent but not integral to the text." .

:notice                                 a rdf:Property ;
                                            rdfs:label "notice" ;
                                            rdf:member :sections ;
                                            htu:usage "[[http://www.w3.org/TR/html5/sections.html#the-section-element section]], [[http://www.w3.org/TR/html5/grouping-content.html#grouping-content grouping content]]" ;
                                            rdfs:comment "A notification." .

:warning                                a rdf:Property ;
                                            rdfs:label "warning" ;
                                            rdf:member :sections ;
                                            htu:usage "[[http://www.w3.org/TR/html5/sections.html#the-section-element section]], [[http://www.w3.org/TR/html5/grouping-content.html#grouping-content grouping content]]" ;
                                            rdfs:comment "A warning." .



########## reference sections #########


:references                             a rdf:Bag ;
                                            jena:bag-sort "40" ;
                                            dcterms:title "Document reference sections" .

:toc                                    a rdf:Property ;
                                            rdfs:label "toc" ;
                                            rdf:member :references ;                                            
                                            htu:usage "[[http://www.w3.org/TR/html5/content-models.html#sectioning-content-0 sectioning content]]" ;
                                            rdfs:comment "A table of contents, typically appearing in the work's frontmatter, or at the beginning of a section." .
					
:loi                                    a rdf:Property ;
                                            rdfs:label "loi" ;
                                            rdf:member :references ;
                                            htu:usage "[[http://www.w3.org/TR/html5/content-models.html#sectioning-content-0 sectioning content]]" ;
                                            rdfs:comment "A listing if of illustrations included in the work." .

:lot                                    a rdf:Property ;
                                            rdfs:label "lot" ;
                                            rdf:member :references ;
                                            htu:usage "[[http://www.w3.org/TR/html5/content-models.html#sectioning-content-0 sectioning content]]" ;
                                            rdfs:comment "A listing of tables included in the work." .
										
:appendix                               a rdf:Property ;
                                            rdfs:label "appendix" ;
                                            rdf:member :references ;
                                            htu:usage "[[http://www.w3.org/TR/html5/content-models.html#sectioning-content-0 sectioning content]]" ;
                                            rdfs:comment "Supplemental information." .

:index                                  a rdf:Property ;
                                            rdfs:label "index" ;
                                            rdf:member :references ;
                                            htu:usage "[[http://www.w3.org/TR/html5/content-models.html#sectioning-content-0 sectioning content]]" ;
                                            rdfs:comment "A detailed list, usually arranged alphabetically, of the specific information in a publication." .

:colophon                               a rdf:Property ;
                                            rdfs:label "colophon" ;
                                            rdf:member :references ;                                            
                                            htu:usage "[[http://www.w3.org/TR/html5/content-models.html#sectioning-content-0 sectioning content]], [[http://www.w3.org/TR/html5/grouping-content.html#grouping-content grouping content]]" ;
                                            rdfs:comment "A brief description usually located at the end of a publication, describing production notes relevant to the edition." .


:landmarks                               a rdf:Property ;
                                            rdfs:label "landmarks" ;
                                            rdf:member :references ;
                                            htu:usage "[[http://www.w3.org/TR/html5/content-models.html#sectioning-content-0 sectioning content]]" ;                                            
                                            rdfs:comment "A collection of references to well-known/recurring components within the publication" .


########## glossaries #########

:glossaries                             a rdf:Bag ;
                                            jena:bag-sort "43" ;
                                            rdf:member :references ;
                                            dcterms:title "Glossaries" .

:glossary                               a rdf:Property ;
                                            rdfs:label "glossary" ;
                                            rdf:member :glossaries ;
                                            htu:usage "[[http://www.w3.org/TR/html5/grouping-content.html#the-dl-element dl]], [[http://www.w3.org/TR/html5/content-models.html#sectioning-content-0 sectioning content]]" ;
                                            jena:prop-sort "10";
                                            rdfs:comment "An alphabetical list of terms in a particular domain of knowledge, with the definitions for those terms." .

:glossterm                              a rdf:Property ;
                                            rdfs:label "glossterm" ;
                                            rdf:member :glossaries ;
                                            role:scope :glossary ;
                                            htu:usage "When the element on which the property appears is a [[http://www.w3.org/TR/html5/grouping-content.html#the-dt-element dt]] element within a [[http://www.w3.org/TR/html5/grouping-content.html#the-dl-element dl]] element marked with the [[#glossary]] property, then the glossterm property on the given dt element is implied." ;                                            
                                            jena:prop-sort "20";
                                            rdfs:comment "A glossary term." .
					
:glossdef                               a rdf:Property ;
                                            rdfs:label "glossdef" ;
                                            role:scope :glossary ;
                                            rdf:member :glossaries ;
                                            htu:usage "When the element on which the property appears a [[http://www.w3.org/TR/html5/grouping-content.html#the-dd-element dd]] element within a [[http://www.w3.org/TR/html5/grouping-content.html#the-dl-element dl]] element marked with the [[#glossary]] property, then the glossdef property on the given dd element is implied. When the element context is a [[http://www.w3.org/TR/html5/sections.html#the-dt-element dd]] element and no explicit glossterm link is provided, then the term that this glossdef participates in defining is located in the nearest preceding [[http://www.w3.org/TR/html5/sections.html#the-dt-element dt]] element sibling. " ;
                                            jena:prop-sort "30";
                                            rdfs:comment "The definition of a [[#glossterm term in a glossary]]." .
                                                                                                                                   

########## bibliographies #########

:bibliographies                          a rdf:Bag ;
                                            jena:bag-sort "46" ;
                                            rdf:member :references ;
                                            dcterms:title "Bibliographies" .

:bibliography                           a rdf:Property ;
                                            rdfs:label "bibliography" ;
                                            rdf:member :bibliographies ;
                                            htu:usage "[[http://www.w3.org/TR/html5/content-models.html#sectioning-content-0 sectioning content]]" ;
                                            rdfs:comment "A list of works cited." .

:biblioentry                            a rdf:Property ;
                                            rdfs:label "biblioentry" ;
                                            rdf:member :bibliographies ;
                                            role:scope :bibliography ;
                                            htu:usage "[[http://www.w3.org/TR/html5/grouping-content.html#grouping-content grouping content]]" ;
                                            rdfs:comment "An entry in a [[#bibliography]]." .


########## preliminary #########

:preliminary                            a rdf:Bag ;
                                            jena:bag-sort "50" ;                                            
                                            dcterms:title "Preliminary sections and components" ;
                                            dcterms:description "Preliminary sections and components, typically occuring in the publication frontmatter." .

:title-page                             a rdf:Property ;
                                            rdfs:label "titlepage" ;
                                            rdf:member :preliminary ;
                                            htu:usage "[[http://www.w3.org/TR/html5/sections.html#the-section-element section]], [[http://www.w3.org/TR/html5/grouping-content.html#grouping-content grouping content]]" ;
                                            rdfs:comment "The title page of the work." .

:halftitle-page                         a rdf:Property ;
                                            rdfs:label "halftitlepage" ;
                                            rdf:member :preliminary ;
                                            htu:usage "[[http://www.w3.org/TR/html5/sections.html#the-section-element section]], [[http://www.w3.org/TR/html5/grouping-content.html#grouping-content grouping content]]" ;
                                            rdfs:comment "The half title page of the work." .

:copyright-page                         a rdf:Property ;
                                            rdfs:label "copyright-page" ;
                                            rdf:member :preliminary ;
                                            htu:usage "[[http://www.w3.org/TR/html5/sections.html#the-section-element section]], [[http://www.w3.org/TR/html5/grouping-content.html#grouping-content grouping content]]" ;
                                            rdfs:comment "The copyright page of the work." .

:acknowledgments                        a rdf:Property ;
                                            rdfs:label "acknowledgments" ;
                                            rdf:member :preliminary ;
                                            htu:usage "[[http://www.w3.org/TR/html5/sections.html#the-section-element section]], [[http://www.w3.org/TR/html5/grouping-content.html#grouping-content grouping content]]" ;
                                            rdfs:comment "A passage containing acknowledgments to entities involved in the realization of the work." .

:imprint                                a rdf:Property ;
                                            rdfs:label "imprint" ;
                                            rdf:member :preliminary ;
                                            htu:usage "[[http://www.w3.org/TR/html5/sections.html#the-section-element section]], [[http://www.w3.org/TR/html5/grouping-content.html#grouping-content grouping content]]" ;
                                            rdfs:comment "Information relating to the publication or distribution of the work." .

:imprimatur                             a rdf:Property ;
                                            rdfs:label "imprimatur" ;
                                            rdf:member :preliminary ;
                                            htu:usage "[[http://www.w3.org/TR/html5/sections.html#the-section-element section]], [[http://www.w3.org/TR/html5/grouping-content.html#grouping-content grouping content]]" ;
                                            rdfs:comment "A formal statement authorizing the publication of the work." .

:contributors                           a rdf:Property ;
                                            rdfs:label "contributors" ;
                                            rdf:member :preliminary ;
                                            htu:usage "[[http://www.w3.org/TR/html5/sections.html#the-section-element section]], [[http://www.w3.org/TR/html5/grouping-content.html#grouping-content grouping content]]" ;
                                            rdfs:comment "A list of contributors to the work." .

:other-credits                          a rdf:Property ;
                                            rdfs:label "other-credits" ;
                                            rdf:member :preliminary ;
                                            htu:usage "[[http://www.w3.org/TR/html5/sections.html#the-section-element section]], [[http://www.w3.org/TR/html5/grouping-content.html#grouping-content grouping content]]" ;
                                            rdfs:comment "Acknowledgments of previously published parts of the work, illustration credits, and permission to quote from copyrighted material." .

:errata                                 a rdf:Property ;
                                            rdfs:label "errata" ;
                                            rdf:member :preliminary ;
                                            htu:usage "[[http://www.w3.org/TR/html5/sections.html#the-section-element section]], [[http://www.w3.org/TR/html5/sections.html#the-aside-element aside]], [[http://www.w3.org/TR/html5/grouping-content.html#grouping-content grouping content]]" ;
                                            rdfs:comment "Publication errata, in printed works typically a loose sheet inserted by hand; sometimes a bound page." .

:dedication                             a rdf:Property ;
                                            rdfs:label "dedication" ;
                                            rdf:member :preliminary ;
                                            htu:usage "[[http://www.w3.org/TR/html5/sections.html#the-section-element section]], [[http://www.w3.org/TR/html5/grouping-content.html#grouping-content grouping content]]" ;
                                            rdfs:comment "An inscription addressed to one or several particular person(s)." .


		
############ complementary ##########

:asides                                 a rdf:Bag ;
                                            jena:bag-sort "60" ;
                                            dcterms:title "Complementary content" .

:sidebar                                a rdf:Property ;
                                            rdfs:label "sidebar" ;
                                            rdfs:subPropertyOf xhv:complementary ;
                                            rdf:member :asides ;
                                            htu:usage "[[http://www.w3.org/TR/html5/sections.html#the-aside-element aside]]" ;
                                            rdfs:comment "Secondary or supplementary content, typically formatted as an inset or box." .

:practice                               a rdf:Property ;
                                            rdfs:label "practice" ;
                                            rdfs:subPropertyOf xhv:complementary ;
                                            rdf:member :asides ;
                                            htu:usage "[[http://www.w3.org/TR/html5/sections.html#the-aside-element aside]]" ;
                                            rdfs:comment "A review exercise or sample." .

:marginalia                             a rdf:Property ;
                                            rdfs:label "marginalia" ;
                                            rdfs:subPropertyOf xhv:complementary ;
                                            rdf:member :asides ;
                                            htu:usage "[[http://www.w3.org/TR/html5/sections.html#the-aside-element aside]], [[http://www.w3.org/TR/html5/content-models.html#phrasing-content phrasing content]]" ;
                                            rdfs:comment "Marginalia." .

:annotation                             a rdf:Property ;
                                            rdfs:label "annotation" ;
                                            rdfs:subPropertyOf xhv:complementary ;
                                            rdf:member :asides ;
                                            htu:usage "[[http://www.w3.org/TR/html5/sections.html#the-aside-element aside]], [[http://www.w3.org/TR/html5/content-models.html#phrasing-content phrasing content]]" ;
                                            rdfs:comment "Explanatory information about passages in the work." .

:help                                   a rdf:Property ;
                                            rdfs:label "help" ;
                                            rdfs:subPropertyOf xhv:complementary ;
                                            rdf:member :asides ;
                                            htu:usage "[[http://www.w3.org/TR/html5/sections.html#the-aside-element aside]], [[http://www.w3.org/TR/html5/content-models.html#phrasing-content phrasing content]]" ;
                                            rdfs:comment "Instructions/advice to the reader on using the work." .

############# notes ##############

:notes                                  a rdf:Bag ;
                                            jena:bag-sort "70" ;
                                            dcterms:title "Notes" .

:note                                   a rdf:Property ;
                                            rdfs:label "note" ;
                                            rdf:member :notes ;
                                            htu:usage "On the [[http://www.w3.org/TR/html5/sections.html#the-aside-element aside]] element when identifying a single note, or on descendants of sectioning content when identifying individual notes in a group (refer to [[#footnotes footnotes]] and [[#rearnotes rearnotes]])." ;
                                            jena:prop-sort "10" ;
                                            rdfs:comment "A [[#footnote]] or a [[#rearnote]], linked from the main text via a note reference." .

:footnote                               a rdf:Property ;
                                            rdfs:label "footnote" ;
                                            rdfs:subPropertyOf :note ;
                                            rdf:member :notes ;
                                            rdfs:seeAlso :footnotes;
                                            htu:usage "On the [[http://www.w3.org/TR/html5/sections.html#the-aside-element aside]] element when identifying a single footnote, or on descendants of sectioning content when identifying individual footnotes in a group (refer to [[#footnotes footnotes]] and [[#rearnotes rearnotes]]). " ;
                                            jena:prop-sort "20" ;
                                            rdfs:comment "A note appearing at the bottom of a page." .

:rearnote                               a rdf:Property ;
                                            rdfs:label "rearnote" ;
                                            rdfs:subPropertyOf :note ;
                                            rdf:member :notes ;
                                            rdfs:seeAlso :rearnotes;
                                            htu:usage "On the [[http://www.w3.org/TR/html5/sections.html#the-aside-element aside]] element when identifying a single rearnote, or on descendants of sectioning content when identifying individual rearnotes in a group (refer to [[#footnotes footnotes]] and [[#rearnotes rearnotes]])." ;
                                            jena:prop-sort "30" ;
                                            rdfs:comment "A note appearing in the rear (backmatter) of the work, or at the end of a section." .


:footnotes                              a rdf:Property ;
                                            rdfs:label "footnotes" ;
                                            rdfs:seeAlso :footnote;
                                            rdf:member :notes ;
                                            htu:usage "[[http://www.w3.org/TR/html5/content-models.html#sectioning-content-0 sectioning content]]" ;
                                            jena:prop-sort "40" ;
                                            rdfs:comment "A collection of notes appearing at the bottom of a page." .

:rearnotes                              a rdf:Property ;
                                            rdfs:label "rearnotes" ;
                                            rdf:member :notes ;
                                            rdfs:seeAlso :rearnote ;
                                            htu:usage "[[http://www.w3.org/TR/html5/content-models.html#sectioning-content-0 sectioning content]]" ;
                                            jena:prop-sort "50" ;
                                            rdfs:comment "A collection of notes appearing at the rear (backmatter) of the work, or at the end of a section." .



############## headings ##############


:headings                               a rdf:Bag ;
                                            jena:bag-sort "80" ;
                                            dcterms:title "Headings" .
					
:bridgehead                             a rdf:Property;
                                            rdfs:label "bridgehead" ;
                                            rdf:member :headings ;
                                            htu:usage "[[http://www.w3.org/TR/html5/Overview.html#flow-content-0 Flow content]], typically [[http://www.w3.org/TR/html5/Overview.html#the-p-element p]], [[http://www.w3.org/TR/html5/Overview.html#the-div-element div]] or [[http://www.w3.org/TR/html5/Overview.html#the-span-element span]]" ;
                                            rdfs:comment "A structurally insignificant heading that does not contribute to the hierarchical structure of the work." .



############### titles ##############
:titles                                 a rdf:Bag ;
                                            jena:bag-sort "90" ;
                                            dcterms:title "Titles" .

:title                                  a rdf:Property ;
                                            rdfs:label "title" ;
                                            rdf:member :titles ;
                                            htu:usage "[[http://www.w3.org/TR/html5/sections.html#the-h1-h2-h3-h4-h5-and-h6-elements h1, h2, h3, h4, h5, h6]], [[http://www.w3.org/TR/html5/sections.html#the-hgroup-element hgroup]]. This property should only appear once within the document scope." ;
                                            jena:prop-sort "10";
                                            rdfs:comment "The title of the work, or, when used in the context of a [[#fulltitle]], the primary part of the full title." .

:halftitle                              a rdf:Property ;
                                            rdfs:label "halftitle" ;
                                            rdfs:subPropertyOf :title ;
                                            rdf:member :titles ;
                                            htu:usage "[[http://www.w3.org/TR/html5/sections.html#the-h1-h2-h3-h4-h5-and-h6-elements h1, h2, h3, h4, h5, h6]], [[http://www.w3.org/TR/html5/sections.html#the-hgroup-element hgroup]]. This property should only appear once within the document scope." ;
                                            jena:prop-sort "20";                                            
                                            rdfs:comment "The title appearing on the first page of a work or immediately before the text." .

:fulltitle                              a rdf:Property ;
                                            rdfs:label "fulltitle" ;
                                            rdfs:subPropertyOf :title ;
                                            rdf:member :titles ;
                                            owl:sameAs dcterms:title;
                                            htu:usage "[[http://www.w3.org/TR/html5/sections.html#the-h1-h2-h3-h4-h5-and-h6-elements h1, h2, h3, h4, h5, h6]], [[http://www.w3.org/TR/html5/sections.html#the-hgroup-element hgroup]]. This property should only appear once within the document scope." ;
                                            jena:prop-sort "30";                                            
                                            rdfs:comment "The full title of the work, either simple, in which case it is identical to [[#title]], or compound, in which case it consists of a [[#title]] and a [[#subtitle]]." .

:subtitle                               a rdf:Property;
                                            rdfs:label "subtitle" ;
                                            rdfs:subPropertyOf :title ;
                                            rdf:member :titles ;
                                            htu:usage "[[http://www.w3.org/TR/html5/sections.html#the-h1-h2-h3-h4-h5-and-h6-elements h1, h2, h3, h4, h5, h6]], [[http://www.w3.org/TR/html5/sections.html#the-hgroup-element hgroup]]" ;
                                            jena:prop-sort "40";
                                            rdfs:comment "An explanatory or alternate title for the work." .

:covertitle                             a rdf:Property;
                                            rdfs:label "covertitle" ;
                                            rdfs:subPropertyOf :title ;
                                            rdf:member :titles ;
                                            htu:usage "[[http://www.w3.org/TR/html5/sections.html#the-h1-h2-h3-h4-h5-and-h6-elements h1, h2, h3, h4, h5, h6]], [[http://www.w3.org/TR/html5/sections.html#the-hgroup-element hgroup]]. This property should only appear once within the document scope." ;
                                            jena:prop-sort "50";                                            
                                            rdfs:comment "The title of the work as displayed on the work's cover." .


############# document text #############


:document-text                          a rdf:Bag ;
                                            jena:bag-sort "100" ;
                                            dcterms:title "Document text" ;
                                            dcterms:description "Terms for describing components at the phrasing level." .

:keyword                                a rdf:Property ;
                                            rdfs:label "keyword" ;
                                            rdf:member :document-text ;
                                            htu:usage "[[http://www.w3.org/TR/html5/content-models.html#phrasing-content-0 phrasing content]]" ;
                                            rdfs:comment "A key word or phrase." .

:topic-sentence                         a rdf:Property ;
                                            rdfs:label "topic-sentence" ;
                                            rdf:member :document-text ;
                                            htu:usage "[[http://www.w3.org/TR/html5/content-models.html#phrasing-content-0 phrasing content]]" ;
                                            rdfs:comment "A phrase or sentence serving as an introductory summary of the containing paragraph." .

:concluding-sentence                    a rdf:Property ;
                                            rdfs:label "concluding-sentence" ;
                                            rdf:member :document-text ;
                                            htu:usage "[[http://www.w3.org/TR/html5/content-models.html#phrasing-content-0 phrasing content]]" ;
                                            rdfs:comment "A phrase or sentence serving as a concluding summary of the containing paragraph." .




############# references ###############


:links                                  a rdf:Bag ;
                                            jena:bag-sort "130" ;
                                            dcterms:title "References" .

#:reference                              a rdf:Property ;
#                                            rdfs:label "reference" ;
#                                            rdf:member :links ;
#                                            rdfs:comment "A reference to another information entity - a resource, fragment, concept, or notion." .
#
:noteref                                a rdf:Property ;
                                            rdfs:label "noteref" ;
                                            rdfs:subPropertyOf xhv:link ;
                                            rdf:member :links ;
                                            htu:usage "[[http://www.w3.org/TR/html5/text-level-semantics.html#the-a-element a]]" ;
                                            rdfs:comment "A reference to a note, typically appearing a superscripted symbol in the main body of text" ;
                                            rdfs:seeAlso :note .

:annoref                                a rdf:Property ;
                                            rdfs:label "annoref" ;
                                            rdfs:subPropertyOf xhv:link ;
                                            rdf:member :links ;
                                            htu:usage "[[http://www.w3.org/TR/html5/text-level-semantics.html#the-a-element a]]" ;
                                            rdfs:comment "A reference to an annotation" ;
                                            rdfs:seeAlso :annotation .

#:citation                               a rdf:Property ;
#                                            rdfs:label "citation" ;
#                                            rdfs:subPropertyOf xhv:link ;
#                                            rdf:member :links ;
#                                            htu:usage "As a value of the [[http://www.w3.org/TR/html5/links.html#attr-hyperlink-rel rel]] attribute on the [[http://www.w3.org/TR/html5/text-level-semantics.html#the-a-element a]] element" ;
#                                            rdfs:comment "A reference to a bibliographic work, resolving to an entry in a directly or indirectly identified bibliography." ;
#                                            rdfs:seeAlso :bibliography .


############## pagination ##############


:pagination                             a rdf:Bag ;
                                            jena:bag-sort "140" ;
                                            dcterms:title "Pagination" .

:pagebreak                              a rdf:Property ;
                                            rdfs:label "pagebreak" ;
                                            rdf:member :pagination ;
                                            htu:usage "[[http://www.w3.org/TR/html5/content-models.html#phrasing-content Phrasing]] and [[http://www.w3.org/TR/html5/content-models.html#flow-content Flow]] content, where the value of the carrying elements title attribute takes precedence over element content for the purposes of representing the pagebreak value" ;
                                            rdfs:comment "A (sometimes valued) separator denoting the position before which a break between two contiguous pages occurs in a statically paginated media." .

:page-list                              a rdf:Property ;
                                            rdfs:label "page-list" ;
                                            rdf:member :pagination ; 
                                            htu:usage "[[http://www.w3.org/TR/html5/content-models.html#sectioning-content-0 sectioning content]]" ;
                                            rdfs:comment "A list of references to [[#pagebreak pagebreaks]] in a statically paginated media" .


#:page-header                            a rdf:Property ;
#                                            rdfs:label "page-header" ;
#                                            rdf:member :pagination ;
#                                            rdfs:comment "Material, separate from the main body of text, appearing at the top of a printed page." .
#
#:page-footer                            a rdf:Property ;
#                                            rdfs:label "page-footer" ;
#                                            rdf:member :pagination ;
#                                            rdfs:comment "Material, separate from the main body of text, appearing at the bottom of a printed page." .
#
#:recto                                  a rdf:Property ;
#                                            rdfs:label "recto" ;
#                                            rdf:member :pagination ;
#                                            rdfs:comment "The front side of a page." .
#
#:verso                                  a rdf:Property ;
#                                            rdfs:label "verso" ;
#                                            rdf:member :pagination ;
#                                            rdfs:comment "The back side of a page." .




############## tables ##############


:tables                             a rdf:Bag ;
                                            jena:bag-sort "150" ;
                                            dcterms:title "Tables" .

:table                              a rdf:Property ;
                                            rdfs:label "table" ;
                                            rdf:member :tables ;
                                            jena:prop-sort "10";
                                            htu:usage "Deprecated"; 
                                            mou:usage "Identifies a [[../../30/spec/epub30-mediaoverlays.html#sec-smil-seq-elem seq]] or [[../../30/spec/epub30-mediaoverlays.html#sec-smil-par-elem par]] as an escapable or skippable table structure." ;
                                            rdfs:comment "A structure containing data or content laid out in tabular form." .

:table-row                          a rdf:Property ;
                                            rdfs:label "table-row" ;
                                            rdf:member :tables ;
                                            jena:prop-sort "20";
                                            htu:usage "Deprecated" ;
                                            mou:usage "Identifies a [[../../30/spec/epub30-mediaoverlays.html#sec-smil-seq-elem seq]] or [[../../30/spec/epub30-mediaoverlays.html#sec-smil-par-elem par]] as an escapable or skippable table row." ;
                                            rdfs:comment "A row of data or content in a tabular structure." .

:table-cell                        a rdf:Property ;
                                            rdfs:label "table-cell" ;
                                            rdf:member :tables ;
                                            jena:prop-sort "30";
                                            htu:usage "Deprecated" ; 
                                            mou:usage "Identifies a [[../../30/spec/epub30-mediaoverlays.html#sec-smil-seq-elem seq]] or [[../../30/spec/epub30-mediaoverlays.html#sec-smil-par-elem par]] as an escapable or skippable table cell." ;
                                            rdfs:comment "A single cell of tabular data or content." .




############## lists ##############


:lists                             a rdf:Bag ;
                                            jena:bag-sort "160" ;
                                            dcterms:title "Lists" .

:list                              a rdf:Property ;
                                            rdfs:label "list" ;
                                            rdf:member :lists ;
                                            jena:prop-sort "10";
                                            htu:usage "Deprecated" ;
                                            mou:usage "Identifies a [[../../30/spec/epub30-mediaoverlays.html#sec-smil-seq-elem seq]] or [[../../30/spec/epub30-mediaoverlays.html#sec-smil-par-elem par]] as an escapable or skippable list structure." ;
                                            rdfs:comment "A structure that contains an enumeration of related content items." .

:list-item                         a rdf:Property ;
                                            rdfs:label "list-item" ;
                                            rdf:member :lists ;
                                            jena:prop-sort "20";
                                            htu:usage "Deprecated" ;
                                            mou:usage "Identifies a [[../../30/spec/epub30-mediaoverlays.html#sec-smil-seq-elem seq]] or [[../../30/spec/epub30-mediaoverlays.html#sec-smil-par-elem par]] as an escapable or skippable list item." ;
                                            rdfs:comment "A single item in an enumeration." .

